src/Iris/Std/Classes.lean
@@ -10,18 +10,18 @@ abbrev Relation (α : Type) := α → α → Prop
 
 
 /-- Require that a relation `R` on `a` is reflexive. -/
-class Reflexive (R : Relation α) where
+class Reflexive (R : Relation α) : Prop where
   refl {x : α} : R x x
 export Reflexive (refl)
 attribute [simp] refl
 
 /-- Require that a relation `R` on `α` is transitive. -/
-class Transitive (R : Relation α) where
+class Transitive (R : Relation α) : Prop where
   trans {x y z : α} : R x y → R y z → R x z
 export Transitive (trans)
 
 /-- Require that a relation `R` on `α` is a preorder, i.e. that it is reflexive and transitive. -/
-class Preorder (R : Relation α) extends Reflexive R, Transitive R
+class Preorder (R : Relation α) extends Reflexive R, Transitive R : Prop
 
 
 /-- Require that a binary function `f` on `α` is idempotent in a relation `R` on `α`. -/
